{$f(x) = \dfrac{x^3+2x^2+x}{x^2-x-2}$}
{$f(x) = \dfrac{x^3+2x^2+x}{x^{2} -x-2} = \dfrac{x(x+1)}{x - 2} \, x \neq -1$\\
Domain: $(-\infty, -1) \cup (-1, 2) \cup (2, \infty)$\\
$x$-intercept:  $(0,0)$\\
$y$-intercept:  $(0,0)$\\
Vertical asymptote: $x = 2$\\
As $x \rightarrow 2^{-}, f(x) \rightarrow -\infty$\\
As $x \rightarrow 2^{+}, f(x) \rightarrow \infty$\\
Hole at $(-1,0)$ \\
Slant asymptote: $y = x+3$ \\
As $x \rightarrow -\infty$, the graph is below $y=x+3$ \\
As $x \rightarrow \infty$, the graph is above $y=x+3$

\begin{center}
\myincludegraphics{figures/RationalsGraphics/RationalGraphs-29}
\end{center}}