{$f(x) = \dfrac{2x - 1}{-2x^{2} - 5x + 3}$}
{$f(x) = \dfrac{2x - 1}{-2x^{2} - 5x + 3} = -\dfrac{2x - 1}{(2x - 1)(x + 3)}$\\
Domain: $(-\infty, -3) \cup (-3, \frac{1}{2}) \cup (\frac{1}{2}, \infty)$\\
No $x$-intercepts\\
$y$-intercept: $(0, -\frac{1}{3})$\\
$f(x) = \dfrac{-1}{x + 3}, \; x \neq \frac{1}{2}$\\
Hole in the graph at $(\frac{1}{2}, -\frac{2}{7})$\\
Vertical asymptote: $x = -3$\\
As $x \rightarrow -3^{-}, \; f(x) \rightarrow \infty$\\
As $x \rightarrow -3^{+}, \; f(x) \rightarrow -\infty$\\
Horizontal asymptote: $y = 0$\\
As $x \rightarrow -\infty, \; f(x) \rightarrow 0^{+}$\\
As $x \rightarrow \infty, \; f(x) \rightarrow 0^{-}$


\begin{center}
\myincludegraphics{figures/RationalsGraphics/RationalGraphs-21}
\end{center}}