{$f(x) = \dfrac{2x^{2} + 5x - 3}{3x + 2}$}
{$f(x) = \dfrac{2x^{2} + 5x - 3}{3x + 2}$\\
Domain: $\left(-\infty, -\frac{2}{3}\right) \cup \left(-\frac{2}{3}, \infty\right)$\\
Vertical asymptote: $x = -\frac{2}{3}$\\
As $x \rightarrow -\frac{2}{3}^{-}, f(x) \rightarrow \infty$\\
As $x \rightarrow -\frac{2}{3}^{+}, f(x) \rightarrow -\infty$\\
No holes in the graph \\
Slant asymptote:  $y = \frac{2}{3}x + \frac{11}{9}$ \\
As $x \rightarrow  -\infty$, the graph is above  $y = \frac{2}{3}x + \frac{11}{9}$\\
As $x \rightarrow \infty$, the graph is below $y = \frac{2}{3}x + \frac{11}{9}$ }
