{$f(x) = \dfrac{x^2-x}{3-x}$}
{$f(x) = \dfrac{x^2-x}{3-x} = \dfrac{x(x-1)}{3-x}$\\
Domain: $(-\infty, 3) \cup (3, \infty)$\\
$x$-intercepts:  $(0,0)$, $(1,0)$\\
$y$-intercept:  $(0,0)$\\
Vertical asymptote: $x = 3$\\
As $x \rightarrow 3^{-}, f(x) \rightarrow \infty$\\
As $x \rightarrow 3^{+}, f(x) \rightarrow -\infty$\\
Slant asymptote: $y = -x-2$ \\
As $x \rightarrow -\infty$, the graph is above $y=-x-2$\\
As $x \rightarrow \infty$, the graph is below $y=-x-2$

\begin{center}
\myincludegraphics{figures/RationalsGraphics/RationalGraphs-28}
\end{center}}