{$f(x) = \dfrac{4x}{x^2-4}$}
{$f(x) = \dfrac{4x}{x^{2} -4} = \dfrac{4x}{(x + 2)(x - 2)}$\\
Domain: $(-\infty, -2) \cup (-2, 2) \cup (2, \infty)$\\
Vertical asymptotes: $x = -2, x = 2$\\
As $x \rightarrow -2^{-}, f(x) \rightarrow -\infty$\\
As $x \rightarrow -2^{+}, f(x) \rightarrow \infty$\\
As $x \rightarrow 2^{-}, f(x) \rightarrow -\infty$\\
As $x \rightarrow 2^{+}, f(x) \rightarrow \infty$\\
No holes in the graph\\
Horizontal asymptote: $y = 0$ \\
As $x \rightarrow -\infty, f(x) \rightarrow 0^{-}$\\
As $x \rightarrow \infty, f(x) \rightarrow 0^{+}$}