{$f(x) = \dfrac{x^2-x-12}{x^2+x-6}$}
{$f(x) = \dfrac{x^2-x-12}{x^{2} +x - 6} = \dfrac{x-4}{x - 2} \, x \neq -3$\\
Domain: $(-\infty, -3) \cup (-3, 2) \cup (2, \infty)$\\
$x$-intercept:  $(4,0)$\\
$y$-intercept:  $(0,2)$\\
Vertical asymptote: $x = 2$\\
As $x \rightarrow 2^{-}, f(x) \rightarrow \infty$\\
As $x \rightarrow 2^{+}, f(x) \rightarrow -\infty$\\
Hole at $\left(-3, \frac{7}{5} \right)$ \\
Horizontal asymptote: $y = 1$ \\
As $x \rightarrow -\infty, f(x) \rightarrow 1^{+}$\\
As $x \rightarrow \infty, f(x) \rightarrow 1^{-}$


\begin{center}
\myincludegraphics{figures/RationalsGraphics/RationalGraphs-25}
\end{center}}