{\footnote{Once you've done the six-step procedure, use a computer or graphing calculator to graph this function on the viewing window $[0, 12] \times [0, 0.25]$.  What do you see?} $f(x) = \dfrac{x^{2} - 2x + 1}{x^{3} + x^{2} - 2x}$ }
{$f(x) = \dfrac{x^{2} - 2x + 1}{x^{3} + x^{2} - 2x}$\\
Domain: $(-\infty, -2) \cup (-2, 0) \cup (0, 1) \cup (1, \infty)$\\
$f(x) = \dfrac{x - 1}{x(x + 2)}, \; x \neq 1$\\
No $x$-intercepts\\
No $y$-intercepts\\
Vertical asymptotes: $x = -2$ and $x = 0$\\
As $x \rightarrow -2^{-}, \; f(x) \rightarrow -\infty$\\
As $x \rightarrow -2^{+}, \; f(x) \rightarrow \infty$\\
As $x \rightarrow 0^{-}, \; f(x) \rightarrow \infty$\\
As $x \rightarrow 0^{+}, \; f(x) \rightarrow -\infty$\\
Hole in the graph at $(1, 0)$\\
Horizontal asymptote: $y = 0$\\
As $x \rightarrow -\infty, \; f(x) \rightarrow 0^{-}$\\
As $x \rightarrow \infty, \; f(x) \rightarrow 0^{+}$


\begin{center}
\myincludegraphics{figures/RationalsGraphics/RationalGraphs-32}
\end{center}}
