{$f(x) = \dfrac{-x^{3} + 4x}{x^{2} - 9}$}
{$f(x) = \dfrac{-x^{3} + 4x}{x^{2} - 9} = \dfrac{-x^{3} + 4x}{(x-3)(x+3)} $\\
Domain: $(-\infty, -3) \cup (-3, 3) \cup (3, \infty)$\\
Vertical asymptotes: $x = -3$, $x=3$\\
As $x \rightarrow -3^{-}, f(x) \rightarrow \infty$\\
As $x \rightarrow -3^{+}, f(x) \rightarrow -\infty$\\
As $x \rightarrow 3^{-}, f(x) \rightarrow \infty$\\
As $x \rightarrow 3^{+}, f(x) \rightarrow -\infty$\\
No holes in the graph \\
Slant asymptote: $y=-x$ \\
As $x \rightarrow -\infty$, the graph is above $y=-x$\\
As $x \rightarrow \infty$, the graph is below $y=-x$}