{$f(x) = \dfrac{3x^2-5x-2}{x^2-9}$}
{$f(x) = \dfrac{3x^2-5x-2}{x^{2} -9} = \dfrac{(3x+1)(x-2)}{(x + 3)(x - 3)}$\\
Domain: $(-\infty, -3) \cup (-3, 3) \cup (3, \infty)$\\
Vertical asymptotes: $x = -3, x = 3$\\
As $x \rightarrow -3^{-}, f(x) \rightarrow \infty$\\
As $x \rightarrow -3^{+}, f(x) \rightarrow -\infty$\\
As $x \rightarrow 3^{-}, f(x) \rightarrow -\infty$\\
As $x \rightarrow 3^{+}, f(x) \rightarrow \infty$\\
No holes in the graph\\
Horizontal asymptote: $y = 3$ \\
As $x \rightarrow -\infty, f(x) \rightarrow 3^{+}$\\
As $x \rightarrow \infty, f(x) \rightarrow 3^{-}$}