{$f(x) = \dfrac{x^2-x-6}{x+1}$}
{$f(x) = \dfrac{x^2-x-6}{x+1} = \dfrac{(x-3)(x+2)}{x+1}$\\
Domain: $(-\infty, -1) \cup (-1, \infty)$\\
$x$-intercepts:  $(-2,0)$, $(3,0)$\\
$y$-intercept:  $(0,-6)$\\
Vertical asymptote: $x = -1$\\
As $x \rightarrow -1^{-}, f(x) \rightarrow \infty$\\
As $x \rightarrow -1^{+}, f(x) \rightarrow -\infty$\\
Slant asymptote: $y = x-2$ \\
As $x \rightarrow -\infty$, the graph is above $y=x-2$\\
As $x \rightarrow \infty$, the graph is below $y=x-2$


\begin{center}
\myincludegraphics{figures/RationalsGraphics/RationalGraphs-27}
\end{center}}
