{$f(x) = \dfrac{-5x^{4} - 3x^{3} + x^{2} - 10}{x^{3} - 3x^{2} + 3x - 1}$}
{$f(x) = \dfrac{-5x^{4} - 3x^{3} + x^{2} - 10}{x^{3} - 3x^{2} + 3x - 1}$ \\ $\phantom{f(x)} = \dfrac{-5x^{4} - 3x^{3} + x^{2} - 10}{(x-1)^3} $ \\
Domain: $(-\infty, 1) \cup (1, \infty)$\\
Vertical asymptotes: $x = 1$\\
As $x \rightarrow 1^{-}, f(x) \rightarrow \infty$\\
As $x \rightarrow 1^{+}, f(x) \rightarrow -\infty$\\
No holes in the graph \\
Slant asymptote: $y=-5x-18$ \\
 As $x \rightarrow -\infty$, the graph is above $y=-5x-18$ \\
As $x \rightarrow \infty$, the graph is below $y=-5x-18$}