{$f(x) = \dfrac{x}{x^{2} + x - 12}$}
{$f(x) = \dfrac{x}{x^{2} + x - 12} = \dfrac{x}{(x - 3)(x + 4)}$\\
Domain: $(-\infty, -4) \cup (-4, 3) \cup (3, \infty)$\\
$x$-intercept: $(0, 0)$\\
$y$-intercept: $(0, 0)$\\
Vertical asymptotes: $x = -4$ and $x = 3$\\
As $x \rightarrow -4^{-}, \; f(x) \rightarrow -\infty$\\
As $x \rightarrow -4^{+}, \; f(x) \rightarrow \infty$\\
As $x \rightarrow 3^{-}, \; f(x) \rightarrow -\infty$\\
As $x \rightarrow 3^{+}, \; f(x) \rightarrow \infty$\\
Horizontal asymptote: $y = 0$\\
As $x \rightarrow -\infty, \; f(x) \rightarrow 0^{-}$\\
As $x \rightarrow \infty, \; f(x) \rightarrow 0^{+}$



\begin{center}
\myincludegraphics{figures/RationalsGraphics/RationalGraphs-22}
\end{center}}