{$f(x) = \dfrac{x}{x^{2} + x - 12}$}
{$f(x) = \dfrac{x}{x^{2} + x - 12} = \dfrac{x}{(x + 4)(x - 3)}$\\
Domain: $(-\infty, -4) \cup (-4, 3) \cup (3, \infty)$\\
Vertical asymptotes: $x = -4, x = 3$\\
As $x \rightarrow -4^{-}, f(x) \rightarrow -\infty$\\
As $x \rightarrow -4^{+}, f(x) \rightarrow \infty$\\
As $x \rightarrow 3^{-}, f(x) \rightarrow -\infty$\\
As $x \rightarrow 3^{+}, f(x) \rightarrow \infty$\\
No holes in the graph\\
Horizontal asymptote: $y = 0$ \\
As $x \rightarrow -\infty, f(x) \rightarrow 0^{-}$\\
As $x \rightarrow \infty, f(x) \rightarrow 0^{+}$}