{$f(x) =  \dfrac{2x}{x^2-4}$, $g(x) =\sqrt{1-x}$ }
{For  $f(x) = \frac{2x}{x^2-4}$ and $g(x) =\sqrt{1-x}$ 

\begin{itemize}

\item  $(g \circ f)(x) =\sqrt{\frac{x^2-2x-4}{x^2-4}}$, domain: $\left(-\infty, -2\right) \cup \left[1-\sqrt{5}, 2\right) \cup \left[1+\sqrt{5}, \infty\right)$

\item  $(f \circ g)(x) = -\frac{2\sqrt{1-x}}{x+3}$, domain: $\left(-\infty, -3\right) \cup \left(-3, 1\right]$

\item  $(f \circ f)(x) = \frac{4x-x^3}{x^4-9x^2+16}$, domain: $\left(-\infty, -\frac{1+\sqrt{17}}{2}\right) \cup \left(-\frac{1+\sqrt{17}}{2}, -2\right) \cup \left(-2, \frac{1-\sqrt{17}}{2}\right) \cup \left(\frac{1-\sqrt{17}}{2}, \frac{-1+\sqrt{17}}{2}\right) \cup \left(\frac{-1+\sqrt{17}}{2}, 2\right) \cup \left(2, \frac{1+\sqrt{17}}{2} \right) \cup \left(\frac{1+\sqrt{17}}{2}, \infty\right)$

\end{itemize}}